@prefix werewolves:     <http://www.utc.fr/werewolves#> .
@prefix skos:    <http://www.w3.org/2004/02/skos/core#> .
@prefix foaf:    <http://xmlns.com/foaf/0.1/> .
@prefix owl:     <http://www.w3.org/2002/07/owl#> .
@prefix rdf:     <http://www.w3.org/1999/02/22-rdf-syntax-ns#> .
@prefix rdfs:    <http://www.w3.org/2000/01/rdf-schema#> .
	
werewolves:Role
	a owl:Class ;
	rdfs:subClassOf foaf:Agent ;
	rdfs:comment "A role in the Werewolves of Millers Hollow game." ;
	rdfs:label "Role" .
		
		
werewolves:Villager
	a werewolves:Role ;
	rdfs:comment "The default role." ;
	rdfs:label "VILLAGER" .
	
werewolves:Werewolf
	a werewolves:Role ;
	rdfs:comment "The werewolf role." ;
	rdfs:label "WEREWOLF" .
	
werewolves:Cupid
	a werewolves:Role ;
	rdfs:comment "The cupid role who can make two people fall in love." ;
	rdfs:label "CUPID" .
	
werewolves:Thief
	a werewolves:Role ;
	rdfs:comment "The thief who can choose between two roles at the beginning of the game." ;
	rdfs:label "THIEF" .
	
werewolves:Guardian
	a werewolves:Role ;
	rdfs:comment "The guardian can protect one person every night." ;
	rdfs:label "GUARDIAN" .
	
werewolves:Clairvoyant
	a werewolves:Role ;
	rdfs:comment "The clairvoyant can see the role of a player every night." ;
	rdfs:label "CLAIRVOYANT" .
	
werewolves:Witch
	a werewolves:Role ;
	rdfs:comment "The witch has two pots: one to revive someone, one to make that person die." ;
	rdfs:label "WITCH" .
	
werewolves:WhiteWolf
	a werewolves:Role ;
	rdfs:comment "The white wolf can kill werewolves and villagers." ;
	rdfs:label "WHITE_WOLF" .
	
werewolves:Raven
	a werewolves:Role ;
	rdfs:comment "The raven can point someone has suspicious every day." ;
	rdfs:label "RAVEN" .
	
werewolves:FlutePlayer
	a werewolves:Role ;
	rdfs:comment "The flute player can charm two players every night." ;
	rdfs:label "FLUTE_PLAYER" .
	
werewolves:Hunter
	a werewolves:Role ;
	rdfs:comment "The hunter can kill someone when he dies." ;
	rdfs:label "HUNTER" .
	
werewolves:Scapegoat
	a werewolves:Role ;
	rdfs:comment "The scapegoat will be hung instead of someone else if several people have the same number of voices." ;
	rdfs:label "SCAPEGOAT" .
	
werewolves:VillageIdiot
	a werewolves:Role ;
	rdfs:comment "The village idiot can not be hung, he is an idiot, he can't be dangerous." ;
	rdfs:label "VILLAGE_IDIOT" .
	
werewolves:VillageSage
	a werewolves:Role ;
	rdfs:comment "The sage can survive to one attack of the wolves." ;
	rdfs:label "VILLAGE_SAGE" .	
	
	
	
werewolves:NbVillagers
	a owl:Property ;
	rdf:subProperty owl:OntologyProperty .
	
werewolves:NbWerewolves
	a owl:Property ;
	rdf:subProperty owl:OntologyProperty .
		


werewolves:GameComposition
	a owl:Class ;
	rdfs:subClassOf foaf:Group ;
	rdfs:comment "A possible composition of a Werewolves of Millers Hollow game." ;
	rdfs:label "Composition".
	
	
werewolves:Composition9A
	a werewolves:GameComposition ;
	owl:cardinality 9 ;
	rdfs:comment "A composition for 9 players with 11 roles for more possibilities and uncertainty.";
	foaf:knows werewolves:Villager ;
	rdfs:subClassOf [ a werewolves:NbVillagers ;
		owl:cardinality 3;
	];
	foaf:knows werewolves:Werewolf ;
	rdfs:subClassOf [ a werewolves:NbWerewolves ;
		owl:cardinality 4;
	];
	foaf:knows werewolves:Guardian ;
	foaf:knows werewolves:Witch ;
	foaf:knows werewolves:Cupid ;
	foaf:knows werewolves:Clairvoyant .
	
	
werewolves:Composition9B
	a werewolves:GameComposition ;
	owl:cardinality 9 ;
	rdfs:comment "A composition for 9 players with 11 roles for more possibilities and uncertainty.";
	foaf:knows werewolves:Villager ;
	rdfs:subClassOf [ a werewolves:NbVillagers ;
		owl:cardinality 3;
	];
	foaf:knows werewolves:Werewolf ;
	rdfs:subClassOf [ a werewolves:NbWerewolves ;
		owl:cardinality 3;
	];
	foaf:knows werewolves:Guardian ;
	foaf:knows werewolves:Witch ;
	foaf:knows werewolves:Hunter ;
	foaf:knows werewolves:Cupid ;
	foaf:knows werewolves:Clairvoyant .
	